coq/ZF/Meta/Test/Decl/Set/Pair.v
@@ -2,11 +2,12 @@ Require Import Coq.Lists.List.
 Require Import Coq.Strings.String.
 
 Require Import ZF.Meta.Ctx.
-Require Import ZF.Meta.Term.Decl.
 Require Import ZF.Meta.Env.
+Require Import ZF.Meta.Proof.Decl.
+Require Import ZF.Meta.Syntax.
+Require Import ZF.Meta.Term.Decl.
 Require Import ZF.Meta.Term.HasTyDecl.
 Require Import ZF.Meta.Term.HasTy.
-Require Import ZF.Meta.Term.Syntax.
 Require Import ZF.Meta.Ty.
 
 Import ListNotations.
@@ -27,21 +28,54 @@ Definition IsPairOf : Decl :=
                (Equal (Var 0) (Var 3))
                (Equal (Var 0) (Var 2)))))) |}.
 
-(* Definition pair (a b:U) : U := The (IsPairOf a b).                           *)
-Definition pair : Decl :=
+(* The existence proof declaration states that some set is a pair of a and b.   *)
+Definition pairExists : Proof.Decl.Decl :=
+  {| Proof.Decl.para  := [TySet; TySet];
+     Proof.Decl.concl :=
+       Ex VarTySet
+         (App
+           (IdentT "IsPairOf" [Var 2; Var 1])
+           (Var 0));
+     Proof.Decl.body  := None |}.
+
+(* The uniqueness proof declaration states that any two such sets are equal.    *)
+Definition pairUnique : Proof.Decl.Decl :=
+  {| Proof.Decl.para  := [TySet; TySet];
+     Proof.Decl.concl :=
+       All VarTySet
+         (All VarTySet
+           (Imp
+             (App
+               (IdentT "IsPairOf" [Var 3; Var 2])
+               (Var 1))
+             (Imp
+               (App
+                 (IdentT "IsPairOf" [Var 3; Var 2])
+                 (Var 0))
+               (Equal (Var 1) (Var 0)))));
+     Proof.Decl.body  := None |}.
+
+(* Definition pair (a b:U) : U := Def (IsPairOf a b) exists unique.             *)
+Definition pair : Term.Decl.Decl :=
   {| para := [TySet; TySet];
      res  := TySet;
      body := Some
-       (The
-         (App
-           (Ident "IsPairOf" [Var 2; Var 1])
-           (Var 0))) |}.
+       (Def
+         (IdentT "IsPairOf" [Var 1; Var 0])
+         (IdentP "pairExists" [Var 1; Var 0])
+         (IdentP "pairUnique" [Var 1; Var 0])) |}.
 
 (* Environment.                                                                 *)
 
-Definition env : Env := Env.fromListT
-  [ ("IsPairOf"%string, IsPairOf)
-  ; ("pair"%string    , pair)
+Definition env : Env := Env.unions
+  [ Env.fromListT
+      [ ("IsPairOf"%string  , IsPairOf)
+      ; ("pair"%string      , pair)
+      ]
+  ; Env.fromListP
+      [ ("pairExists"%string, pairExists)
+      ; ("pairUnique"%string, pairUnique)
+      ]
   ].
 
 (* Body checks.                                                                 *)
@@ -55,18 +89,72 @@ Proof.
   - apply HasTyOr; apply HasTyEqual; apply (HasTyVar _ _ _ TySet); reflexivity.
 Qed.
 
-(* The declaration body for pair denotes the set satisfying IsPairOf.           *)
-Proposition pairCheckBody : HasTyDecl env pair.
+(* The existence proof declaration conclusion is a well-sorted proposition.     *)
+Proposition pairExistsCheckConcl :
+  HasTy env (Proof.Decl.ctx pairExists) (Proof.Decl.concl pairExists) TyProp.
 Proof.
   (* Proof by Hermes + gpt 5.5                                                  *)
-  apply HasTyThe, HasTyApp.
-  - apply HasTyIdent with [TySet; TySet]. 1: reflexivity.
+  apply HasTyEx, HasTyApp.
+  - apply HasTyIdentT with [TySet; TySet]. 1: reflexivity.
     apply HasTysCons.
     + apply (HasTyVar _ _ _ TySet). reflexivity.
     + apply HasTysCons.
       * apply (HasTyVar _ _ _ TySet). reflexivity.
       * apply HasTysNil.
   - apply (HasTyVar _ _ _ TySet). reflexivity.
+Qed.
+
+(* The uniqueness proof declaration conclusion is a well-sorted proposition.    *)
+Proposition pairUniqueCheckConcl :
+  HasTy env (Proof.Decl.ctx pairUnique) (Proof.Decl.concl pairUnique) TyProp.
+Proof.
+  (* Proof by Hermes + gpt 5.5                                                  *)
+  apply HasTyAll, HasTyAll, HasTyImp.
+  - apply HasTyApp.
+    + apply HasTyIdentT with [TySet; TySet]. 1: reflexivity.
+      apply HasTysCons.
+      * apply (HasTyVar _ _ _ TySet). reflexivity.
+      * apply HasTysCons.
+        -- apply (HasTyVar _ _ _ TySet). reflexivity.
+        -- apply HasTysNil.
+    + apply (HasTyVar _ _ _ TySet). reflexivity.
+  - apply HasTyImp.
+    + apply HasTyApp.
+      * apply HasTyIdentT with [TySet; TySet]. 1: reflexivity.
+        apply HasTysCons.
+        -- apply (HasTyVar _ _ _ TySet). reflexivity.
+        -- apply HasTysCons.
+           ++ apply (HasTyVar _ _ _ TySet). reflexivity.
+           ++ apply HasTysNil.
+      * apply (HasTyVar _ _ _ TySet). reflexivity.
+    + apply HasTyEqual; apply (HasTyVar _ _ _ TySet); reflexivity.
+Qed.
+
+(* The declaration body for pair denotes a set backed by proof references.      *)
+Proposition pairCheckBody : HasTyDecl env pair.
+Proof.
+  (* Proof by Hermes + gpt 5.5                                                  *)
+  apply HasTyDef.
+  - apply HasTyIdentT with [TySet; TySet]. 1: reflexivity.
+    apply HasTysCons.
+    + apply (HasTyVar _ _ _ TySet). reflexivity.
+    + apply HasTysCons.
+      * apply (HasTyVar _ _ _ TySet). reflexivity.
+      * apply HasTysNil.
+  - apply HasTyIdentP with pairExists. 1: reflexivity.
+    + apply HasTysCons.
+      * apply (HasTyVar _ _ _ TySet). reflexivity.
+      * apply HasTysCons.
+        -- apply (HasTyVar _ _ _ TySet). reflexivity.
+        -- apply HasTysNil.
+    + apply pairExistsCheckConcl.
+  - apply HasTyIdentP with pairUnique. 1: reflexivity.
+    + apply HasTysCons.
+      * apply (HasTyVar _ _ _ TySet). reflexivity.
+      * apply HasTysCons.
+        -- apply (HasTyVar _ _ _ TySet). reflexivity.
+        -- apply HasTysNil.
+    + apply pairUniqueCheckConcl.
 Qed.
 
 (* Identifier checks.                                                           *)
@@ -76,11 +164,11 @@ Proposition IsPairOfCheckIdent : forall (e:Env) (G:Ctx) (m n:nat),
   e "IsPairOf"%string = Some IsPairOf ->
   typeOf G m = Some TySet ->
   typeOf G n = Some TySet ->
-  HasTy e G (Ident "IsPairOf" [Var m; Var n]) TyClass.
+  HasTy e G (IdentT "IsPairOf" [Var m; Var n]) TyClass.
 Proof.
   (* Proof by Hermes + gpt 5.5                                                  *)
   intros e G m n H1 H2 H3.
-  apply HasTyIdent with [TySet; TySet].
+  apply HasTyIdentT with [TySet; TySet].
   - unfold Env.toSigs. rewrite H1. reflexivity.
   - apply HasTysCons.
     + apply HasTyVar. assumption.
@@ -94,11 +182,11 @@ Proposition pairCheckIdent : forall (e:Env) (G:Ctx) (m n:nat),
   e "pair"%string = Some pair ->
   typeOf G m = Some TySet ->
   typeOf G n = Some TySet ->
-  HasTy e G (Ident "pair" [Var m; Var n]) TySet.
+  HasTy e G (IdentT "pair" [Var m; Var n]) TySet.
 Proof.
   (* Proof by Hermes + gpt 5.5                                                  *)
   intros e G m n H1 H2 H3.
-  apply HasTyIdent with [TySet; TySet].
+  apply HasTyIdentT with [TySet; TySet].
   - unfold Env.toSigs. rewrite H1. reflexivity.
   - apply HasTysCons.
     + apply HasTyVar. assumption.
