coq/ZF/Meta/Proof/Decl.v
@@ -1,8 +1,7 @@
 Require Import Coq.Lists.List.
 
 Require Import ZF.Meta.Ctx.
-Require Import ZF.Meta.Proof.Syntax.
-Require Import ZF.Meta.Term.Syntax.
+Require Import ZF.Meta.Syntax.
 Require Import ZF.Meta.Ty.
 
 Import ListNotations.
