coq/ZF/Meta/Syntax.v
@@ -1,0 +1,31 @@
+Require Import Coq.Lists.List.
+Require Import Coq.Strings.String.
+Require Import ZF.Meta.Ty.
+
+Import ListNotations.
+
+Inductive Term : Type :=
+| Bot     : Term
+| Top     : Term
+| Var     : nat    -> Term
+| IdentT  : string -> list Term -> Term
+| Elem    : Term   -> Term      -> Term
+| Leq     : Term   -> Term      -> Term
+| Geq     : Term   -> Term      -> Term
+| Lt      : Term   -> Term      -> Term
+| Gt      : Term   -> Term      -> Term
+| Equal   : Term   -> Term      -> Term
+| NotEq   : Term   -> Term      -> Term
+| Imp     : Term   -> Term      -> Term
+| Iff     : Term   -> Term      -> Term
+| And     : Term   -> Term      -> Term
+| Or      : Term   -> Term      -> Term
+| Not     : Term   -> Term
+| All     : VarTy  -> Term      -> Term
+| Ex      : VarTy  -> Term      -> Term
+| Lam     : Term   -> Term
+| App     : Term   -> Term      -> Term
+| Def     : Term   -> Proof     -> Proof     -> Term
+with Proof : Type :=
+| IdentP : string -> list Term -> Proof
+.
