coq/ZF/Meta/Test/Axiom/Extensionality.v
@@ -1,6 +1,6 @@
 Require Import ZF.Meta.Ctx.
 Require Import ZF.Meta.Env.
-Require Import ZF.Meta.Term.Syntax.
+Require Import ZF.Meta.Syntax.
 Require Import ZF.Meta.Term.HasTy.
 Require Import ZF.Meta.Ty.
 
