coq/ZF/Meta/Test/Class/Equiv.v
@@ -3,7 +3,7 @@ Require Import Coq.Strings.String.
 
 Require Import ZF.Meta.Ctx.
 Require Import ZF.Meta.Term.HasTy.
-Require Import ZF.Meta.Term.Syntax.
+Require Import ZF.Meta.Syntax.
 Require Import ZF.Meta.Ty.
 
 Require Import ZF.Meta.Test.Decl.Class.Equiv.
@@ -15,7 +15,7 @@ Import ListNotations.
 (* Proposition Refl : forall (P:Class), equiv P P.                              *)
 Definition Refl : Term :=
   All VarTyClass
-    (Ident "equiv" [Var 0; Var 0]).
+    (IdentT "equiv" [Var 0; Var 0]).
 
 (* Proposition EquivCompat : forall A B C D,                                    *)
 (* equiv A C -> equiv B D -> equiv A B -> equiv C D.                            *)
@@ -25,12 +25,12 @@ Definition EquivCompat : Term :=
       (All VarTyClass
         (All VarTyClass
           (Imp
-            (Ident "equiv" [Var 3; Var 1])
+            (IdentT "equiv" [Var 3; Var 1])
             (Imp
-              (Ident "equiv" [Var 2; Var 0])
+              (IdentT "equiv" [Var 2; Var 0])
               (Imp
-                (Ident "equiv" [Var 3; Var 2])
-                (Ident "equiv" [Var 1; Var 0]))))))).
+                (IdentT "equiv" [Var 3; Var 2])
+                (IdentT "equiv" [Var 1; Var 0]))))))).
 
 (* Proposition EquivCompatL : forall A B C,                                     *)
 (* equiv A C -> equiv A B -> equiv C B.                                         *)
@@ -39,10 +39,10 @@ Definition EquivCompatL : Term :=
     (All VarTyClass
       (All VarTyClass
         (Imp
-          (Ident "equiv" [Var 2; Var 0])
+          (IdentT "equiv" [Var 2; Var 0])
           (Imp
-            (Ident "equiv" [Var 2; Var 1])
-            (Ident "equiv" [Var 0; Var 1]))))).
+            (IdentT "equiv" [Var 2; Var 1])
+            (IdentT "equiv" [Var 0; Var 1]))))).
 
 (* Proposition EquivCompatR : forall A B C,                                     *)
 (* equiv B C -> equiv A B -> equiv A C.                                         *)
@@ -51,18 +51,18 @@ Definition EquivCompatR : Term :=
     (All VarTyClass
       (All VarTyClass
         (Imp
-          (Ident "equiv" [Var 1; Var 0])
+          (IdentT "equiv" [Var 1; Var 0])
           (Imp
-            (Ident "equiv" [Var 2; Var 1])
-            (Ident "equiv" [Var 2; Var 0]))))).
+            (IdentT "equiv" [Var 2; Var 1])
+            (IdentT "equiv" [Var 2; Var 0]))))).
 
 (* Proposition Sym : forall P Q, equiv P Q -> equiv Q P.                        *)
 Definition Sym : Term :=
   All VarTyClass
     (All VarTyClass
       (Imp
-        (Ident "equiv" [Var 1; Var 0])
-        (Ident "equiv" [Var 0; Var 1]))).
+        (IdentT "equiv" [Var 1; Var 0])
+        (IdentT "equiv" [Var 0; Var 1]))).
 
 (* Proposition Tran : forall P Q R,                                             *)
 (* equiv P Q -> equiv Q R -> equiv P R.                                         *)
@@ -71,18 +71,18 @@ Definition Tran : Term :=
     (All VarTyClass
       (All VarTyClass
         (Imp
-          (Ident "equiv" [Var 2; Var 1])
+          (IdentT "equiv" [Var 2; Var 1])
           (Imp
-            (Ident "equiv" [Var 1; Var 0])
-            (Ident "equiv" [Var 2; Var 0]))))).
+            (IdentT "equiv" [Var 1; Var 0])
+            (IdentT "equiv" [Var 2; Var 0]))))).
 
 (* Proposition NotSym : forall P Q, ~ equiv P Q -> ~ equiv Q P.                 *)
 Definition NotSym : Term :=
   All VarTyClass
     (All VarTyClass
       (Imp
-        (Not (Ident "equiv" [Var 1; Var 0]))
-        (Not (Ident "equiv" [Var 0; Var 1])))).
+        (Not (IdentT "equiv" [Var 1; Var 0]))
+        (Not (IdentT "equiv" [Var 0; Var 1])))).
 
 (* Proposition EqualToClass : forall a b,                                       *)
 (* a = b <-> equiv (toClass a) (toClass b).                                     *)
@@ -91,8 +91,8 @@ Definition EqualToClass : Term :=
     (All VarTySet
       (Iff
         (Equal (Var 1) (Var 0))
-        (Ident "equiv"
-          [Ident "toClass" [Var 1]; Ident "toClass" [Var 0]]))).
+        (IdentT "equiv"
+          [IdentT "toClass" [Var 1]; IdentT "toClass" [Var 0]]))).
 
 (* Proposition NotEqualToClass : forall a b,                                    *)
 (* a <> b <-> ~ equiv (toClass a) (toClass b).                                  *)
@@ -102,8 +102,8 @@ Definition NotEqualToClass : Term :=
       (Iff
         (NotEq (Var 1) (Var 0))
         (Not
-          (Ident "equiv"
-            [Ident "toClass" [Var 1]; Ident "toClass" [Var 0]])))).
+          (IdentT "equiv"
+            [IdentT "toClass" [Var 1]; IdentT "toClass" [Var 0]])))).
 
 (* Proposition NotCompat : forall P Q R S,                                      *)
 (* equiv P Q -> equiv R S -> ~ equiv P R -> ~ equiv Q S.                        *)
@@ -113,12 +113,12 @@ Definition NotCompat : Term :=
       (All VarTyClass
         (All VarTyClass
           (Imp
-            (Ident "equiv" [Var 3; Var 2])
+            (IdentT "equiv" [Var 3; Var 2])
             (Imp
-              (Ident "equiv" [Var 1; Var 0])
+              (IdentT "equiv" [Var 1; Var 0])
               (Imp
-                (Not (Ident "equiv" [Var 3; Var 1]))
-                (Not (Ident "equiv" [Var 2; Var 0])))))))).
+                (Not (IdentT "equiv" [Var 3; Var 1]))
+                (Not (IdentT "equiv" [Var 2; Var 0])))))))).
 
 (* Proposition NotCompatL : forall P Q R,                                       *)
 (* equiv P Q -> ~ equiv P R -> ~ equiv Q R.                                     *)
@@ -127,10 +127,10 @@ Definition NotCompatL : Term :=
     (All VarTyClass
       (All VarTyClass
         (Imp
-          (Ident "equiv" [Var 2; Var 1])
+          (IdentT "equiv" [Var 2; Var 1])
           (Imp
-            (Not (Ident "equiv" [Var 2; Var 0]))
-            (Not (Ident "equiv" [Var 1; Var 0])))))).
+            (Not (IdentT "equiv" [Var 2; Var 0]))
+            (Not (IdentT "equiv" [Var 1; Var 0])))))).
 
 (* Proposition NotCompatR : forall P Q R,                                       *)
 (* equiv P Q -> ~ equiv R P -> ~ equiv R Q.                                     *)
@@ -139,10 +139,10 @@ Definition NotCompatR : Term :=
     (All VarTyClass
       (All VarTyClass
         (Imp
-          (Ident "equiv" [Var 2; Var 1])
+          (IdentT "equiv" [Var 2; Var 1])
           (Imp
-            (Not (Ident "equiv" [Var 0; Var 2]))
-            (Not (Ident "equiv" [Var 0; Var 1])))))).
+            (Not (IdentT "equiv" [Var 0; Var 2]))
+            (Not (IdentT "equiv" [Var 0; Var 1])))))).
 
 (* Proposition typing.                                                          *)
 
@@ -151,7 +151,7 @@ Proposition ReflCheck : HasTy env Ctx.empty Refl TyProp.
 Proof.
   (* Proof by Hermes + gpt 5.5                                                  *)
   apply HasTyAll.
-  apply HasTyIdent with [TyClass; TyClass]. 1: reflexivity.
+  apply HasTyIdentT with [TyClass; TyClass]. 1: reflexivity.
   apply HasTysCons.
   - apply (HasTyVar _ _ _ TyClass). reflexivity.
   - apply HasTysCons.
@@ -219,7 +219,7 @@ Proof.
   (* Proof by Hermes + gpt 5.5                                                  *)
   apply HasTyAll, HasTyAll, HasTyIff.
   - apply HasTyEqual; apply (HasTyVar _ _ _ TySet); reflexivity.
-  - apply HasTyIdent with [TyClass; TyClass]. 1: reflexivity.
+  - apply HasTyIdentT with [TyClass; TyClass]. 1: reflexivity.
     apply HasTysCons.
     + apply toClassCheckIdent; reflexivity.
     + apply HasTysCons.
@@ -235,7 +235,7 @@ Proof.
   apply HasTyAll, HasTyAll, HasTyIff.
   - apply HasTyNotEq; apply (HasTyVar _ _ _ TySet); reflexivity.
   - apply HasTyNot.
-    apply HasTyIdent with [TyClass; TyClass]. 1: reflexivity.
+    apply HasTyIdentT with [TyClass; TyClass]. 1: reflexivity.
     apply HasTysCons.
     + apply toClassCheckIdent; reflexivity.
     + apply HasTysCons.
