coq/ZF/Meta/Test/Decl/Class/Equiv.v
@@ -6,7 +6,7 @@ Require Import ZF.Meta.Term.Decl.
 Require Import ZF.Meta.Env.
 Require Import ZF.Meta.Term.HasTyDecl.
 Require Import ZF.Meta.Term.HasTy.
-Require Import ZF.Meta.Term.Syntax.
+Require Import ZF.Meta.Syntax.
 Require Import ZF.Meta.Ty.
 
 Import ListNotations.
@@ -64,11 +64,11 @@ Qed.
 Proposition toClassCheckIdent : forall (e:Env) (G:Ctx) (n:nat),
   e "toClass"%string = Some toClass ->
   typeOf G n = Some TySet ->
-  HasTy e G (Ident "toClass" [Var n]) TyClass.
+  HasTy e G (IdentT "toClass" [Var n]) TyClass.
 Proof.
   (* Proof by Hermes + gpt 5.5                                                  *)
   intros e G n H1 H2.
-  apply HasTyIdent with [TySet].
+  apply HasTyIdentT with [TySet].
   - unfold Env.toSigs. rewrite H1. reflexivity.
   - apply HasTysCons.
     + apply HasTyVar. assumption.
@@ -80,11 +80,11 @@ Proposition equivCheckIdent : forall (e:Env) (G:Ctx) (m n:nat),
   e "equiv"%string = Some equiv ->
   typeOf G m = Some TyClass ->
   typeOf G n = Some TyClass ->
-  HasTy e G (Ident "equiv" [Var m; Var n]) TyProp.
+  HasTy e G (IdentT "equiv" [Var m; Var n]) TyProp.
 Proof.
   (* Proof by Hermes + gpt 5.5                                                  *)
   intros e G m n H1 H2 H3.
-  apply HasTyIdent with [TyClass; TyClass].
+  apply HasTyIdentT with [TyClass; TyClass].
   - unfold Env.toSigs. rewrite H1. reflexivity.
   - apply HasTysCons.
     + apply HasTyVar. assumption.
@@ -98,7 +98,7 @@ Proposition notEquivCheckIdent : forall (e:Env) (G:Ctx) (m n:nat),
   e "equiv"%string = Some equiv ->
   typeOf G m = Some TyClass ->
   typeOf G n = Some TyClass ->
-  HasTy e G (Not (Ident "equiv" [Var m; Var n])) TyProp.
+  HasTy e G (Not (IdentT "equiv" [Var m; Var n])) TyProp.
 Proof.
   (* Proof by Hermes + gpt 5.5                                                  *)
   intros e G m n H1 H2 H3.
